@prefix :      <http://www.w3.org/2000/01/rdf-schema#> .
@prefix con:   <http://www.w3.org/2000/10/swap/pim/contact#> .
@prefix dc:    <http://purl.org/dc/elements/1.1/> .
@prefix rdfs:  <http://www.w3.org/2000/01/rdf-schema#> .
@prefix doc:   <http://www.w3.org/2000/10/swap/pim/doc#> .
@prefix owl:   <http://www.w3.org/2002/07/owl#> .
@prefix rdf:   <http://www.w3.org/1999/02/22-rdf-syntax-ns#> .

con:child  a    rdf:Property .

con:vacationHome  a  rdf:Property ;
        rdfs:domain  con:Person ;
        rdfs:label   "vacation" ;
        rdfs:range   con:ContactLocation .

con:Female  a   rdfs:Class .

con:organization  rdfs:domain  con:Person .

con:ContactLocation  a  rdfs:Class ;
        rdfs:comment  "A place, or mobile situation, with address, phone number, fax, etc. \n    Related to a person by home, office, etc.\n    Note one person's workplace may be another person's home.\n    A person may have more than one home and more than one workplace.\n    (In practice it sometimes maybe useful with restriucted datasets to\n    assume that this is not the case, when extracting data from other ontologies\n    with no concept of ContactLocation).  Strongly related to a person: \n    in some ways a role that a person can be in." ;
        rdfs:label    "contact point" .

con:fullName  a     rdf:Property ;
        rdfs:label  "full name" .

con:knownAs  a        rdf:Property ;
        rdfs:comment  "A person may be known as various strings.\n\tFor example, an email friendly name string.\n\tIf you have an email from someone using a string as the human-readable phrase,\n\tthen it is reasonable to assume that there are :knownAs that." ;
        rdfs:label    "name" .

con:publicHomePage  rdfs:subPropertyOf  con:homePage .

con:partner  a       rdf:Property ;
        rdfs:domain  con:Person ;
        rdfs:range   con:Person .

con:homePage  a               owl:InverseFunctionalProperty ;
        rdfs:subPropertyOf    con:webPage ;
        con:_addressProperty  con:homePageAddress .

con:departmentName  rdfs:domain  con:Person .

con:fax  a           rdf:Property ;
        rdfs:domain  con:ContactLocation ;
        rdfs:range   con:Fax .

con:emergency  a     rdf:Property ;
        rdfs:domain  con:Person ;
        rdfs:label   "emergency only" ;
        rdfs:range   con:ContactLocation .

con:Address  a  rdfs:Class .

con:webPage  a        rdf:Property ;
        rdfs:comment  "A related web page" ;
        rdfs:label    "web page" .

con:_SubjectToChange  rdfs:label  "subject to change" .

con:Male  a     rdfs:Class .

con:zip  rdfs:subPropertyOf  con:postalCode .

con:Pager  rdfs:subClassOf  con:Phone .

con:street  rdfs:domain  con:Address .

con:mailboxURI  a     owl:InverseFunctionalProperty ;
        rdfs:comment  "mailboxURI is a string.  Use of this is discouraged. Use :mailbox instead " ;
        rdfs:domain   con:SocialEntity ;
        rdfs:range    con:_URI ;
        con:_example  "\n            <rdf:Description xmlns:rdf=\"http://www.w3.org/1999/02/22-rdf-syntax-ns#\" rdf:about=\"http://www.w3.org/2000/10/swap/pim/contact#_Dan\">\n                <con:mailboxURI xmlns:con=\"http://www.w3.org/2000/10/swap/pim/contact#\">mailto:connolly@w3.org</con:mailboxURI>\n            </rdf:Description>\n        "^^rdf:XMLLiteral .

con:firstName  rdfs:domain  con:Person .

con:middleName  rdfs:domain  con:Person .

con:Fax  rdfs:label      "fax" ;
        rdfs:subClassOf  con:Phone .

con:nearestAirport  a  rdf:Property ;
        rdfs:comment  "?X nearestAirport ?Y locates ?X in an international\n   context; for example, for the purpose of organizing a face-to-face\n   meeting of a W3C working group. This property is intended to mitigate\n   privacy risks of giving out detailed contact info." ;
        rdfs:label    "nearest airport" ;
        rdfs:seeAlso  <http://www.w3.org/2001/tag/ilist#httpRange-14> , <http://www.w3.org/2001/sw/WebOnt/webont-airports.rdf> , <http://www.w3.org/2001/sw/Europe/200303/geo/intro.html> , <http://www.perceive.net/pages/page/articles/year/2002/month/12#9> , <http://lists.w3.org/Archives/Public/www-webont-wg/2001Nov/0006.html> .

con:givenName  rdfs:domain  con:Person .

con:title  rdfs:domain  con:Person .

con:postalCode  rdfs:domain  con:Address .

con:assistant  a      rdf:Property ;
        rdfs:comment  "A person (or other agent) who is an assistant to the subject." ;
        rdfs:domain   <http://xmlns.com/foaf/0.1/Agent> ;
        rdfs:label    "assistant" ;
        rdfs:ramge    <http://xmlns.com/foaf/0.1/Agent> .

con:participant  a    rdf:Property ;
        rdfs:comment  "A person (or other agent) who  particpates in an event, meeting, etc." ;
        rdfs:label    "participant" ;
        rdfs:ramge    <http://xmlns.com/foaf/0.1/Agent> .

con:personalSuffix  rdfs:domain  con:Person .

con:sortName  a       rdf:Property ;
        rdfs:comment  "re-arranged for lexicographic ordering; ala Doe, John" ;
        rdfs:label    "sort name" .

con:SocialEntity  a   rdfs:Class ;
        rdfs:comment  "The sort of thing which can have a phone number.\n    Typically a person or an incorporated company, or unincorporated group." .

con:familyName  rdfs:domain  con:Person .

con:middleInitial  rdfs:domain  con:Person .

con:motherTongue  a  rdf:Property ;
        rdfs:domain  con:Person ;
        rdfs:range   con:LanguageCode .

con:country  rdfs:domain  con:Address .

con:street3  rdfs:domain  con:Address .

con:office  a        rdf:Property ;
        rdfs:domain  con:Person ;
        rdfs:label   "work" ;
        rdfs:range   con:ContactLocation .

con:preferredURI  a   rdf:Property ;
        rdfs:comment  "A string which is the URI a person, organization, etc, prefers that people use for them." ;
        rdfs:label    "preferred" .

con:description  a  rdf:Property .

con:personalTitle  rdfs:domain  con:Person .

con:mailbox  a                owl:InverseFunctionalProperty ;
        rdfs:domain           con:SocialEntity ;
        rdfs:range            con:Mailbox ;
        con:_addressProperty  con:mailboxURI ;
        con:_example          "\n            <rdf:Description xmlns:rdf=\"http://www.w3.org/1999/02/22-rdf-syntax-ns#\" rdf:about=\"http://www.w3.org/2000/10/swap/pim/contact#_Dan\">\n                <con:mailbox xmlns:con=\"http://www.w3.org/2000/10/swap/pim/contact#\" rdf:resource=\"mailto:connolly@w3.org\"></con:mailbox>\n            </rdf:Description>\n        "^^rdf:XMLLiteral .

con:emailAddress  a   owl:InverseFunctionalProperty ;
        rdfs:comment  "emailAddress is a string.  Use of this is discouraged. Use :mailbox instead " ;
        rdfs:domain   con:SocialEntity ;
        rdfs:label    "email" ;
        rdfs:range    con:_EmailAddress ;
        con:_example  "\n            <rdf:Description xmlns:rdf=\"http://www.w3.org/1999/02/22-rdf-syntax-ns#\" rdf:about=\"http://www.w3.org/2000/10/swap/pim/contact#_Dan\">\n                <con:emailAddress xmlns:con=\"http://www.w3.org/2000/10/swap/pim/contact#\">connolly@w3.org</con:emailAddress>\n            </rdf:Description>\n        "^^rdf:XMLLiteral .

con:_addressProperty  a  rdf:Property .

<http://www.w3.org/2000/10/swap/pim/contact>
        dc:description         "$Id: contact.rdf,v 1.18 2011/02/01 04:13:21 timbl Exp $" , "\n To illustrate with examples the creation of a schema of RDF properties\n and classes, but using abstract things for people, rather than strings, etc.\n If you have an \"Assistant's phone number\", then really you have an assitant who has\n a phone number - and that is much more useful in general.\n For example, when data about you and your assietnt in merged,\n you will end up with an \"assistant's email\" and the like.\n" ;
        dc:title               "Contact: Utility concepts for everyday life" ;
        doc:creator            <http://www.w3.org/People/Berners-Lee/card#i> ;
        doc:persistencePolicy  [ a               con:_SubjectToChange ;
                                 dc:description  "If you change this, you have to tell the W3C SemWeb AD\n   folk, including Dan Connolly; so agreed 5 Jun 2001.\n   TimBl takes this as being met by a mail to sw-team."
                               ] ;
        doc:rules              <http://www.w3.org/2000/10/swap/pim/contact-rules> .

con:homePageAddress  a  owl:InverseFunctionalProperty ;
        rdfs:comment  "Use is discouraged" .

con:birthday  a      rdf:Property ;
        rdfs:domain  con:SocialEntity ;
        rdfs:range   con:Date .

con:MobilePhone  rdfs:label  "mobile" ;
        rdfs:subClassOf  con:Phone .

con:Phone  a          rdfs:Class ;
        rdfs:comment  "\n    An end-point in the public swiitched telephone system.\n    Anything identified by a URI with tel: scheme is in this class.\n    " ;
        rdfs:label    "tel."@fr , "phone"@en .

con:stateOrProvince  rdfs:domain  con:Address .

con:Person  rdfs:comment  "A person in the normal sense of the word." ;
        rdfs:subClassOf  con:SocialEntity .

con:phone  a         rdf:Property ;
        rdfs:domain  con:ContactLocation ;
        rdfs:range   con:Phone .

con:address  a       rdf:Property ;
        rdfs:domain  con:ContactLocation ;
        rdfs:label   "address"@en ;
        rdfs:range   con:Address .

con:region  a         rdf:Property ;
        rdfs:comment  "The sub-national unit such as state (us),\nprovince (ca), county (uk), d√©partement (fr), and so on" ;
        rdfs:label    "region" .

con:mobile  a        rdf:Property ;
        rdfs:domain  con:Person ;
        rdfs:label   "mobile" ;
        rdfs:range   con:ContactLocation .

con:street2  rdfs:domain  con:Address .

con:home  a          rdf:Property ;
        rdfs:domain  con:Person ;
        rdfs:label   "home" ;
        rdfs:range   con:ContactLocation .

con:lastName  rdfs:domain  con:Person .

con:city  rdfs:domain  con:Address .

doc:persistencePolicy
        rdfs:seeAlso  <http://www.w3.org/1999/10/nsuri> .

con:LanguageCode  a  rdfs:Class .
